\documentclass[fleqn,12pt]{article}
\input{preamble2}
\usepackage{amsmath}
\usepackage[colorlinks]{hyperref}
\setlength{\parindent}{0em}
\setlength{\parskip}{1em}
\begin{document}
\thispagestyle{empty}

\section*{Logic pset 4}

Resources: HLW \href{https://www.jstor.org/stable/j.ctvxrpz0q.6}{Ch 3}
and
\href{https://princeton.hosted.panopto.com/Panopto/Pages/Viewer.aspx?id=748f0cd0-1329-4bd9-9e2a-acbf0155b44c}{Lecture
  6}

Use Conditional Proof (and possibly the previous rules) to prove the
following sequents. Be sure to include dependency numbers in the
leftmost column of your proof.
\begin{enumerate}
\item $P\to Q\:\vdash\: P\to (Q\vee R)$
\item $P\:\vdash\: (P\to\neg P)\to \neg P$
\item $P\to (Q\to R)\:\vdash\: Q\to (P\to R)$  
\item $\vdash\: P\to (P\vee Q)$
\item $\vdash\: P\to ((P\to Q)\to Q)$
\end{enumerate}     

\end{document}


%%% Local Variables:
%%% mode: latex
%%% TeX-master: t
%%% End:
